# RDF Vocabulary document for OSLC Configuration Management

@prefix dcterms:     <http://purl.org/dc/terms/> .
@prefix owl:         <http://www.w3.org/2002/07/owl#> .
@prefix oslc_config: <http://open-services.net/ns/config#> .
@prefix rdf:         <http://www.w3.org/1999/02/22-rdf-syntax-ns#> .
@prefix rdfs:        <http://www.w3.org/2000/01/rdf-schema#> .
@prefix vann:        <http://purl.org/vocab/vann/> .
@prefix vs:          <http://www.w3.org/2003/06/sw-vocab-status/ns#> .


# the vocabulary

oslc_config:
    a owl:Ontology ;
    dcterms:title "OSLC Configuration Management vocabulary" ;
    dcterms:description "The OSLC Configuration Management vocabulary defines terms for versioned resources and configurations of those versioned resources." ;
    rdfs:label "OSLC Configuration Management vocabulary" ;
    vann:preferredNamespacePrefix "oslc_config" ;

    dcterms:source <http://tools.oasis-open.org/version-control/svn/oslc-core/trunk/specs/config/config-vocab.ttl> ;

    # TBD - what should the license and copyright info be here?
    dcterms:license "TBD" ;
    dcterms:dateCopyrighted "2012-2015" .


# Classes

oslc_config:Activity
    a rdfs:Class ;
    rdfs:isDefinedBy oslc_config: ;
    rdfs:label "Activity" ;
    rdfs:comment "An activity is a read-only resource representing a long-running operation, such as recursive baseline or stream creation." .

oslc_config:Baseline
    a rdfs:Class ;
    rdfs:isDefinedBy oslc_config: ;
    rdfs:label "Baseline" ;
    rdfs:subClassOf oslc_config:Configuration ;
    rdfs:comment "An immutable configuration, with immutable contributions and immutable selections of immutable resources. All contributions to this configuration MUST be baselines." .

oslc_config:ChangeSet
    a rdfs:Class ;
    rdfs:isDefinedBy oslc_config: ;
    rdfs:label "ChangeSet" ;
    rdfs:subClassOf oslc_config:Configuration ;
    rdfs:comment "A change set configuration represents a set of changes (including additions and removals) to some other configuration." .

oslc_config:ChangeSetSelections
    a rdfs:Class ;
    rdfs:isDefinedBy oslc_config: ;
    rdfs:label "ChangeSetSelections" ;
    rdfs:subClassOf oslc_config:Selections ;
    rdfs:comment "A resource listing the version resources selected by a change set configuration." .

oslc_config:Component
    a rdfs:Class ;
    rdfs:isDefinedBy oslc_config: ;
    rdfs:label "Component" ;
    rdfs:comment "A unit of organization consisting of a set of versioned resources. Components are the units of configurability, and form reusable assets or building blocks." .

oslc_config:Configuration
    a rdfs:Class ;
    rdfs:isDefinedBy oslc_config: ;
    rdfs:label "Configuration" ;
    rdfs:comment "A configuration identifies a set of versions of resources in a component. Configurations commonly identify exactly one version of each resource in a component. Configurations can also assemble other configurations into a shared context across multiple components." .

oslc_config:ConfigurationSettings
    a rdfs:Class ;
    rdfs:isDefinedBy oslc_config: ;
    rdfs:label "ConfigurationSettings" ;
    rdfs:comment "Information about settings and preferences for a Configuration Management service." .

oslc_config:Contribution
    a rdfs:Class ;
    rdfs:isDefinedBy oslc_config: ;
    rdfs:label "Contribution" ;
    rdfs:comment "A contribution represents the contribution of one configuration to another." .

oslc_config:PersonalConfiguration
    a rdfs:Class ;
    rdfs:isDefinedBy oslc_config: ;
    rdfs:label "PersonalConfiguration" ;
    rdfs:subClassOf oslc_config:Configuration ;
    rdfs:comment "A configuration intended for use by a single agent, rather than shared." .

oslc_config:Selections
    a rdfs:Class ;
    rdfs:isDefinedBy oslc_config: ;
    rdfs:label "Selections" ;
    rdfs:comment "A resource listing the version resources selected by a configuration." .

oslc_config:Removals
    a rdfs:Class ;
    rdfs:isDefinedBy oslc_config: ;
    rdfs:label "Removals" ;
    rdfs:comment "For a change set, the selections to be removed from an overridden configuration." .

oslc_config:RemoveAll
    a rdfs:Class ;
    rdfs:isDefinedBy oslc_config: ;
    rdfs:label "RemovalAll" ;
    rdfs:comment "For a change set, an indicator that all selections in the overriden configuration are to be ignored; all selections are defined by the change set." .

oslc_config:UnboundSelections
    a rdfs:Class ;
    rdfs:isDefinedBy oslc_config: ;
    rdfs:label "UnboundSelections" ;
    rdfs:comment "An indicator that a set of selections are as-yet unbound concept resources as opposed to bound version resources." .

oslc_config:Stream
    a rdfs:Class ;
    rdfs:isDefinedBy oslc_config: ;
    rdfs:label "Stream" ;
    rdfs:subClassOf oslc_config:Configuration ;
    rdfs:comment "A mutable configuration. Contributions to this configuration can be streams or baselines." .

oslc_config:VersionResource
    a rdfs:Class ;
    rdfs:isDefinedBy oslc_config: ;
    rdfs:label "VersionResource" ;
    rdfs:comment "This type is used as a marker for any version resource." .


# Properties

oslc_config:accepts
    a rdf:Property ;
    rdfs:isDefinedBy oslc_config: ;
    rdfs:label "accepts" ;
    rdfs:range oslc_config:Configuration ;
    rdfs:comment "A type of configuration acceptable as a contribution to the subject configuration." .

oslc_config:acceptedBy
    a rdf:Property ;
    rdfs:isDefinedBy oslc_config: ;
    rdfs:label "acceptedBy" ;
    rdfs:range oslc_config:Configuration ;
    rdfs:comment "A type of configuration accepted as a contribution by the subject configuration." .

oslc_config:baselineOfStream
    a rdf:Property ;
    rdfs:isDefinedBy oslc_config: ;
    rdfs:label "baselineOfStream" ;
    rdfs:range oslc_config:Stream ;
    rdfs:comment "The stream from which a baseline was made." .

oslc_config:baselines
    a rdf:Property ;
    rdfs:isDefinedBy oslc_config: ;
    rdfs:label "baselines" ;
    rdfs:comment "A Linked Data Platform Container for baselines of a stream." .

oslc_config:branch
    a rdf:Property ;
    rdfs:isDefinedBy oslc_config: ;
    rdfs:label "branch" ;
    rdfs:comment "Identifies a resource as one for a specific branch or variant of the component." .

oslc_config:committed
    a rdf:Property ;
    rdfs:isDefinedBy oslc_config: ;
    rdfs:label "committed" ;
    rdfs:comment "Date and time a resource was committed, or checked in." .

oslc_config:committer
    a rdf:Property ;
    rdfs:isDefinedBy oslc_config: ;
    rdfs:label "committer" ;
    rdfs:comment "The entity that committed or checked in this resource." .

oslc_config:component
    a rdf:Property ;
    rdfs:isDefinedBy oslc_config: ;
    rdfs:label "component" ;
    rdfs:comment "A reference to a Component resource." .

oslc_config:configuration
    a rdf:Property ;
    rdfs:isDefinedBy oslc_config: ;
    rdfs:label "configuration" ;
    rdfs:comment "A reference to a Configuration resource." .

oslc_config:configurations
    a rdf:Property ;
    rdfs:isDefinedBy oslc_config: ;
    rdfs:label "configurations" ;
    rdfs:comment "A Linked Data Platform Container for configurations of a component." .

oslc_config:configurationSettings
    a rdf:Property ;
    rdfs:isDefinedBy oslc_config: ;
    rdfs:label "configurationSettings" ;
    rdfs:comment "A reference to information about settings and preferences for a Configuration Management service." .

oslc_config:contribution
    a rdf:Property ;
    rdfs:isDefinedBy oslc_config: ;
    rdfs:label "contribution" ;
    rdfs:range oslc_config:Contribution ;
    rdfs:comment "A reference to a Contribution resource." .

oslc_config:contributionOrder
    a rdf:Property ;
    rdfs:isDefinedBy oslc_config: ;
    rdfs:label "contributionOrder" ;
    rdfs:comment "The ordering value for a contribution." .

oslc_config:overrides
    a rdf:Property ;
    rdfs:isDefinedBy oslc_config: ;
    rdfs:label "overrides" ;
    rdfs:comment "A reference to a configuration modified by a change set configuration." .

oslc_config:previousBaseline
    a rdf:Property ;
    rdfs:isDefinedBy oslc_config: ;
    rdfs:label "previousBaseline" ;
    rdfs:range oslc_config:Baseline ;
    rdfs:comment "For a stream or a baseline, a link to the most recent baseline of the same stream." .

oslc_config:progressMessage
    a rdf:Property ;
    rdfs:isDefinedBy oslc_config: ;
    rdfs:label "progressMessage" ;
    rdfs:comment "Text describing the progress of an operation." .

oslc_config:selections
    a rdf:Property ;
    rdfs:isDefinedBy oslc_config: ;
    rdfs:label "selections" ;
    rdfs:range oslc_config:Selections ;
    rdfs:comment "A reference to a Selections resource." .

oslc_config:selects
    a rdf:Property ;
    rdfs:isDefinedBy oslc_config: ;
    rdfs:label "selects" ;
    rdfs:comment "A reference to a selected version resource." .

oslc_config:streams
    a rdf:Property ;
    rdfs:isDefinedBy oslc_config: ;
    rdfs:label "streams" ;
    rdfs:comment "A Linked Data Platform Container for streams created from a baseline." .

oslc_config:versionId
    a rdf:Property ;
    rdfs:isDefinedBy oslc_config: ;
    rdfs:label "versionId" ;
    rdfs:comment "A human-readable version identifier." .


# Obsolete terms

oslc_config:derivedFrom
    a rdf:Property ;
    rdfs:isDefinedBy oslc_config: ;
    rdfs:label "derivedFrom" ;
    vs:term_status "archaic" ;
    rdfs:comment "A resource from which this resource was derived; the use of prov:wasDerivedFrom is preferred." .

oslc_config:mutable
    a rdf:Property ;
    rdfs:isDefinedBy oslc_config: ;
    rdfs:label "mutable" ;
    vs:term_status "archaic" ;
    rdfs:comment "A boolean property indicating whether or not a resource is modifiable; replaced by use of Baseline and Stream types." .


# Individuals

oslc_config:globalConfigurationService
    a rdfs:Resource ;
    rdfs:isDefinedBy oslc_config: ;
    rdfs:label "globalConfigurationService" ;
    rdfs:comment "An oslc:usage value marking a global configuration service." .
