# Copyright 2019 OASIS Open
#
# Licensed under the Apache License, Version 2.0 (the "License");
# you may not use this file except in compliance with the License.
# You may obtain a copy of the License at
#
#     http://www.apache.org/licenses/LICENSE-2.0
#
# Unless required by applicable law or agreed to in writing, software
# distributed under the License is distributed on an "AS IS" BASIS,
# WITHOUT WARRANTIES OR CONDITIONS OF ANY KIND, either express or implied.
# See the License for the specific language governing permissions and
# limitations under the License.


# RDF Vocabulary document for The OSLC Change Management Domain

@prefix oslc_cm: <http://open-services.net/ns/cm#> .
@prefix owl: <http://www.w3.org/2002/07/owl#> .
@prefix dcterms: <http://purl.org/dc/terms/> .
@prefix vann: <http://purl.org/vocab/vann/> .
@prefix rdf: <http://www.w3.org/1999/02/22-rdf-syntax-ns#> .
@prefix rdfs: <http://www.w3.org/2000/01/rdf-schema#> .
@prefix vs: <http://www.w3.org/2003/06/sw-vocab-status/ns#> .

@base <https://tools.oasis-open.org/version-control/svn/oslc-ccm/trunk/specs/change-mgt/change-mgt-vocab.ttl>.

oslc_cm:
  a owl:Ontology ;
  dcterms:title "The OSLC Change Management(CM) Vocabulary" ;
  dcterms:description "All vocabulary URIs defined in the OSLC Change Management (CM) namespace."^^rdf:XMLLiteral ;
  dcterms:source <https://tools.oasis-open.org/version-control/svn/oslc-ccm/trunk/specs/change-mgt/change-mgt-vocab.ttl> ;
  vann:preferredNamespacePrefix "oslc_cm" ;
  rdfs:label "Change Management(CM)" .

# ******** Classes ********

oslc_cm:ChangeRequest
  a rdfs:Class ;
  rdfs:isDefinedBy oslc_cm: ;
  rdfs:label "ChangeRequest" ;
  rdfs:comment "The CM Change Request resource." .

oslc_cm:ChangeNotice
  a rdfs:Class ;
  rdfs:subClassOf oslc_cm:ChangeRequest ;
  rdfs:isDefinedBy oslc_cm: ;
  rdfs:label "ChangeNotice" ;
  rdfs:comment "Represents an assignment notification of a change request. May be used also to bestow authority onto the assigned user to effect the changes." .


oslc_cm:Defect
  a rdfs:Class ;
  rdfs:subClassOf oslc_cm:ChangeRequest ;
  rdfs:isDefinedBy oslc_cm: ;
  rdfs:label "Defect" ;
  rdfs:comment "A software or product defect." .

oslc_cm:Enhancement
  a rdfs:Class ;
  rdfs:subClassOf oslc_cm:ChangeRequest ;
  rdfs:isDefinedBy oslc_cm: ;
  rdfs:label "Enhancement" ;
  rdfs:comment "A request for new functionality." .

oslc_cm:ReviewTask
  a rdfs:Class ;
  rdfs:subClassOf oslc_cm:Task ;
  rdfs:isDefinedBy oslc_cm: ;
  rdfs:label "ReviewTask" ;
  rdfs:comment "A request to make a change and review the change." .

oslc_cm:Task
  a rdfs:Class ;
  rdfs:subClassOf oslc_cm:ChangeRequest ;
  rdfs:isDefinedBy oslc_cm: ;
  rdfs:label "Task" ;
  rdfs:comment "An executable and trackable activity." .


# ******** Properties ********

oslc_cm:authorizer
  a rdf:Property ;
  rdfs:isDefinedBy oslc_cm: ;
  rdfs:label "authorizer" ;
  rdfs:comment "The URI of a resource describing an agent who is responsible authorizing for and/or has authorized effort to be expended to address a set of change requests." .

oslc_cm:parent
  a rdf:Property ;
  rdfs:isDefinedBy oslc_cm: ;
  rdfs:label "parent" ;
  rdfs:comment "The related parent change requests of the subject change request." .

oslc_cm:closeDate
  a rdf:Property ;
  rdfs:isDefinedBy oslc_cm: ;
  rdfs:label "closeDate" ;
  rdfs:comment "The date at which no further activity or work is intended to be conducted." .

oslc_cm:priority
  a rdf:Property ;
  rdfs:isDefinedBy oslc_cm: ;
  rdfs:label "priority" ;
  rdfs:comment """Used to indicate the relative importance of ChangeRequests.
It is likely that the target resource will be an
oslc_cm:Priority.""" .

oslc_cm:severity
  a rdf:Property ;
  rdfs:isDefinedBy oslc_cm: ;
  rdfs:label "severity" ;
  rdfs:comment """Used to indicate the severity or potential impact of a defect.
It is likely that the target resource will be an oslc_cm:Severity.""" .

oslc_cm:relatedChangeRequest
  a rdf:Property ;
  rdfs:isDefinedBy oslc_cm: ;
  rdfs:label "relatedChangeRequest" ;
  rdfs:comment """This relationship is loosely coupled, has no specific
meaning, and can be used to link related change requests. It is likely
that the target resource will be an oslc_cm:ChangeRequest.""" .

oslc_cm:affectsPlanItem
  a rdf:Property ;
  rdfs:isDefinedBy oslc_cm: ;
  rdfs:label "affectsPlanItem" ;
  rdfs:comment """Change request affects a plan item. It is likely that
the target resource will be an oslc_cm:ChangeRequest.""" .

oslc_cm:affectedByDefect
  a rdf:Property ;
  rdfs:isDefinedBy oslc_cm: ;
  rdfs:label "affectedByDefect" ;
  rdfs:comment """Change request is affected by a reported defect. It is
likely that the target resource will be an oslc_cm:Defect.""" .

oslc_cm:tracksRequirement
  a rdf:Property ;
  rdfs:isDefinedBy oslc_cm: ;
  rdfs:label "tracksRequirement" ;
  rdfs:comment """Tracks the associated Requirement or Requirement
ChangeSet resources. It is likely that the target resource will be an
oslc_rm:Requirement.""" .

oslc_cm:implementsRequirement
  a rdf:Property ;
  rdfs:isDefinedBy oslc_cm: ;
  rdfs:label "implementsRequirement" ;
  rdfs:comment """The ChangeRequest implements the associated Requirement. It is likely that the
target resource will be an oslc_rm:Requirement.""" .

oslc_cm:affectsRequirement
  a rdf:Property ;
  rdfs:isDefinedBy oslc_cm: ;
  rdfs:label "affectsRequirement" ;
  rdfs:comment """The ChangeRequest affects a Requirement. It is likely
that the target resource will be an oslc_rm:Requirement.""" .

oslc_cm:tracksChangeSet
  a rdf:Property ;
  rdfs:isDefinedBy oslc_cm: ;
  rdfs:label "tracksChangeSet" ;
  rdfs:comment """Tracks a change set resource. It is likely that the
target resource will be an oslc_config:ChangeSet.""" .

oslc_cm:state
  a rdf:Property ;
  rdfs:isDefinedBy oslc_cm: ;
  rdfs:label "state" ;
  rdfs:comment "Used to indicate the status of the change request." .


# oslc_cm:state allowed values

oslc_cm:State
  a rdfs:Class ;
  rdfs:isDefinedBy oslc_cm: ;
  rdfs:label "State" ;
  rdfs:comment "Defines the possible oslc_cm:state property values." .

oslc_cm:Closed
  a oslc_cm:State ;
  rdfs:isDefinedBy oslc_cm: ;
  rdfs:label "closed" ;
  rdfs:comment "Whether or not the Change Request is completely done, no further fixes or fix verification is needed." .

oslc_cm:Inprogress
  a oslc_cm:State ;
  rdfs:isDefinedBy oslc_cm: ;
  rdfs:label "inprogress" ;
  rdfs:comment "Whether or not the Change Request in a state indicating that active work is occurring." .

oslc_cm:Fixed
  a oslc_cm:State ;
  rdfs:isDefinedBy oslc_cm: ;
  rdfs:label "fixed" ;
  rdfs:comment "Whether or not the Change Request has been fixed." .

oslc_cm:Approved
  a oslc_cm:State ;
  rdfs:isDefinedBy oslc_cm: ;
  rdfs:label "approved" ;
  rdfs:comment "Whether or not the Change Request has been approved." .

oslc_cm:Reviewed
  a oslc_cm:State ;
  rdfs:isDefinedBy oslc_cm: ;
  rdfs:label "reviewed" ;
  rdfs:comment "Whether or not the Change Request has been reviewed." .

oslc_cm:Verified
  a oslc_cm:State ;
  rdfs:isDefinedBy oslc_cm: ;
  rdfs:label "verified" ;
  rdfs:comment "Whether or not the resolution or fix of the Change Request has been verified." .


# Priority allowed values

oslc_cm:Priority
  a rdfs:Class ;
  rdfs:isDefinedBy oslc_cm: ;
  rdfs:label "Priority" ;
  rdfs:comment "Defines the possible oslc_cm:priority property values." .

oslc_cm:High
  a oslc_cm:Priority ;
  rdfs:isDefinedBy oslc_cm: ;
  rdfs:label "High" ;
  rdfs:comment "Highest priority, action on the change request highly recommended." .

oslc_cm:Medium
  a oslc_cm:Priority ;
  rdfs:isDefinedBy oslc_cm: ;
  rdfs:label "Medium" ;
  rdfs:comment "Acting on the change request can wait, but not forever." .

oslc_cm:Low
  a oslc_cm:Priority ;
  rdfs:isDefinedBy oslc_cm: ;
  rdfs:label "Low" ;
  rdfs:comment "Action on the change request can be safely deferred." .

oslc_cm:PriorityUnassigned
  a oslc_cm:Priority ;
  rdfs:isDefinedBy oslc_cm: ;
  rdfs:label "PriorityUnassigned" ;
  rdfs:comment "The priority of the change request is intentionally not set." .



# Severity allowed values

oslc_cm:Severity
  a rdfs:Class ;
  rdfs:isDefinedBy oslc_cm: ;
  rdfs:label "Severity" ;
  rdfs:comment "Defines the possible oslc_cm:severity property values." .

oslc_cm:Blocker
  a oslc_cm:Severity ;
  rdfs:isDefinedBy oslc_cm: ;
  rdfs:label "Blocker" ;
  rdfs:comment "Severe problem. No workaround. Blocks development, test, or usage." .

oslc_cm:Critical
  a oslc_cm:Severity ;
  rdfs:isDefinedBy oslc_cm: ;
  rdfs:label "Critical" ;
  rdfs:comment "Severe problem. No workaround." .

oslc_cm:Major
  a oslc_cm:Severity ;
  rdfs:isDefinedBy oslc_cm: ;
  rdfs:label "Major" ;
  rdfs:comment "Prevents function from being used. There is a workaround." .

oslc_cm:Normal
  a oslc_cm:Severity ;
  rdfs:isDefinedBy oslc_cm: ;
  rdfs:label "Normal" ;
  rdfs:comment "Affects non-critical functionality. There is a workaround." .

oslc_cm:Minor
  a oslc_cm:Severity ;
  rdfs:isDefinedBy oslc_cm: ;
  rdfs:label "Minor" ;
  rdfs:comment "Minimal impact." .

oslc_cm:SeverityUnassigned
  a oslc_cm:Severity ;
  rdfs:isDefinedBy oslc_cm: ;
  rdfs:label "SeverityUnassigned" ;
  rdfs:comment "The severity of the change request is intentionally not set." .


###########################################################################

# Deprecated vocabulary terms:

# Deprecated, use oslc_cm:state instead
oslc_cm:status
  a rdf:Property ;
  rdfs:isDefinedBy oslc_cm: ;
  vs:term_status "archaic" ;
  rdfs:label "status" ;
  rdfs:comment """Used to indicate the status of the change request based
on values defined by the service provider. Most often a read-only
property. It is likely that the target resource will be a string corresponding to an
oslc_cm:State value.""" .


# Properties that were deprecated in CM 2.0, and continue to be deprecated in CM 3.0

oslc_cm:testedByTestCase
  a rdf:Property ;
  rdfs:isDefinedBy oslc_cm: ;
  vs:term_status "archaic" ;
  rdfs:label "testedByTestCase" ;
  rdfs:comment """Test case by which this change request is tested. It is
likely that the target resource will be an oslc_qm:TestCase.""" .

oslc_cm:affectsTestResult
  a rdf:Property ;
  rdfs:isDefinedBy oslc_cm: ;
  vs:term_status "archaic" ;
  rdfs:label "affectsTestResult" ;
  rdfs:comment """Associated resource that is affected by this Change
Request. It is likely that the target resource will be an
oslc_qm:TestResult.""" .

oslc_cm:blocksTestExecutionRecord
  a rdf:Property ;
  rdfs:isDefinedBy oslc_cm: ;
  vs:term_status "archaic" ;
  rdfs:label "blocksTestExecutionRecord" ;
  rdfs:comment """Associated resource that is blocked by this Change
Request. It is likely that the target resource will be an
oslc_qm:TestExecutionRecord.""" .

oslc_cm:relatedTestExecutionRecord
  a rdf:Property ;
  rdfs:isDefinedBy oslc_cm: ;
  vs:term_status "archaic" ;
  rdfs:label "relatedTestExecutionRecord" ;
  rdfs:comment """Related to a test execution resource. It is likely
that the target resource will be an oslc_qm:TestExecutionRecord.""" .

oslc_cm:relatedTestCase
  a rdf:Property ;
  rdfs:isDefinedBy oslc_cm: ;
  vs:term_status "archaic" ;
  rdfs:label "relatedTestCase" ;
  rdfs:comment """Related test case resource. It is likely that the
target resource will be an oslc_qm:TestCase.""" .

oslc_cm:relatedTestPlan
  a rdf:Property ;
  rdfs:isDefinedBy oslc_cm: ;
  vs:term_status "archaic" ;
  rdfs:label "relatedTestPlan" ;
  rdfs:comment """Related test plan resource. It is likely that the
target resource will be an oslc_qm:TestPlan.""" .

oslc_cm:relatedTestScript
  a rdf:Property ;
  rdfs:isDefinedBy oslc_cm: ;
  vs:term_status "archaic" ;
  rdfs:label "relatedTestScript" ;
  rdfs:comment """Related test script resource. It is likely that the
target resource will be an oslc_qm:TestScript.""" .

# Individuals for oslc:usage values to designate specific CM ServiceProvider services

oslc_cm:defect
  a rdfs:Resource ;
  rdfs:isDefinedBy oslc_cm: ;
  rdfs:label "defect" ;
  rdfs:comment "Used to report defects in testing." .

oslc_cm:planItem
  a rdfs:Resource ;
  rdfs:isDefinedBy oslc_cm: ;
  rdfs:label "planItem" ;
  rdfs:comment "Used for associating change requests into plans (project, release, sprint, etc)." .

oslc_cm:task
  a rdfs:Resource ;
  rdfs:isDefinedBy oslc_cm: ;
  rdfs:label "task" ;
  rdfs:comment "Used for associating change requests into executable and track-able items." .

oslc_cm:requirementsChangeRequest
  a rdfs:Resource ;
  rdfs:isDefinedBy oslc_cm: ;
  rdfs:label "requirementsChangeRequest" ;
  rdfs:comment "Used for associating a change request for usage in tracking changes to a Requirements resource." .

# Boolean State Predicate properties used to define a standard set of ChangeRequest states
# These values are usually read-only and calculated to summarize the state of a ChangeRequest
# But servers may allow them to be changed

oslc_cm:closed
  a rdf:Property ;
  rdfs:isDefinedBy oslc_cm: ;
  rdfs:label "closed" ;
  rdfs:comment "Whether or not the Change Request is completely done, no further fixes or fix verification is needed." .

oslc_cm:inProgress
  a rdf:Property ;
  rdfs:isDefinedBy oslc_cm: ;
  rdfs:label "inProgress" ;
  rdfs:comment "Whether or not the Change Request in a state indicating that active work is occurring." .

oslc_cm:fixed
  a rdf:Property ;
  rdfs:isDefinedBy oslc_cm: ;
  rdfs:label "fixed" ;
  rdfs:comment "Whether or not the Change Request has been fixed." .

oslc_cm:approved
  a rdf:Property ;
  rdfs:isDefinedBy oslc_cm: ;
  rdfs:label "approved" ;
  rdfs:comment "Whether or not the Change Request has been approved." .

oslc_cm:reviewed
  a rdf:Property ;
  rdfs:isDefinedBy oslc_cm: ;
  rdfs:label "reviewed" ;
  rdfs:comment "Whether or not the Change Request has been reviewed." .

oslc_cm:verified
  a rdf:Property ;
  rdfs:isDefinedBy oslc_cm: ;
  rdfs:label "verified" ;
  rdfs:comment "Whether or not the resolution or fix of the Change Request has been verified." .
